# 1-10

## Problem Statement

From the definition provided in the book, Ackermann's function is defined as:

$$
\begin{equation}
A(x, y) = \begin{cases}
	0                     &\text{if}\ y = 0 \\
	2y                    &\text{if}\ x = 0 \\
	2                     &\text{if}\ y = 1 \\
	A(x - 1, A(x, y - 1)) &\text{otherwise.}
\end{cases}
\end{equation}
$$

We are asked to solve for $f(n) = A(0, n)$, $g(n) = A(1, n)$, $h(n) = A(2, n)$
in terms of $n$, where $n \in \Z^+$.

## Solution for $f(n)$

$$
f(n) = A(0, n) = 2n
$$

## Solution for $g(n)$

I'm not going to proof this; It's pretty simple to demonstrate this via
induction.

$$
\begin{split}
g(n) &= A(1, n)
	\\ &= A(0, A(1, n - 1))
	\\ &= 2A(1, n - 1)
	\\ &= 2^2 A(1, n - 2)
	\\ &= ...
	\\ &= 2^n
	\\ &= 2 \uparrow n
\end{split}
$$

Where $\uparrow$ denotes Knuth's up-arrow notation.

## Solution for $h(n)$

Same as above. No proofies for you.

$$
\begin{split}
h(n) = A(2, n)
	\\ &= A(1, A(2, n - 1))
	\\ &= 2^{A(2, n - 1)}
	\\ &= 2^{2^{A(2, n - 2)}}
	\\ &= ...
	\\ &= 2 \uparrow \uparrow n
\end{split}
$$

Here, $2 \uparrow \uparrow n = 2^{2 \uparrow \uparrow (n - 1)}$.
